

Lecture 23: Theme 23 (Mon 20 Oct 2025 18:58)

Limit when $x \rightarrow a$

Example 1 (page 155): Calculate $\lim_{x \rightarrow 1} \frac{1}{|x-1|}$

$$\text{We know } |x-1| = \begin{cases} x-1 & (x \geq 1) \\ 1-x & (1 > x) \end{cases}$$

$$\Rightarrow \frac{1}{|x-1|} = \begin{cases} \frac{1}{x-1} & (x > 1) \\ \frac{1}{1-x} & (x < 1) \end{cases}$$

$$\Rightarrow \lim_{x \rightarrow 1^+} \frac{1}{x-1} = +\infty \text{ Explain: } \begin{cases} 1 > 0 \\ \lim_{x \rightarrow 1^+} = 0^+ \end{cases}$$

$$\Rightarrow \lim_{x \rightarrow 1^-} \frac{1}{1-x} = +\infty \text{ Explain: } \begin{cases} 1 > 0 \\ \lim_{x \rightarrow 1^-} = 0^+ \end{cases}$$

$$\Rightarrow \lim_{x \rightarrow 1} = +\infty$$

Example 2 (page 155): Calculate $\lim_{x \rightarrow 0} (1 - \frac{1}{x^2})$.

$$\lim_{x \rightarrow 0^+} (1 - \frac{1}{x^2}) = -\infty$$

$$\lim_{x \rightarrow 0^-} (1 - \frac{1}{x^2}) = -\infty$$

$$\Rightarrow \lim_{x \rightarrow 0} = -\infty$$

Example 1 (page 156): Calculate $\lim_{x \rightarrow 3} (x^2 - 2x + 3)$

Method 1: Nature

$$\begin{aligned} & \lim_{x \rightarrow 3} (x^2 - 2x + 3) \\ &= \lim_{x \rightarrow 3} x^2 - \lim_{x \rightarrow 3} 2x + \lim_{x \rightarrow 3} 3 \\ &= \lim_{x \rightarrow 3} x \cdot \lim_{x \rightarrow 3} x - 2 \lim_{x \rightarrow 3} x + \lim_{x \rightarrow 3} 3 \\ &= 3 \cdot 3 - 2 \cdot 3 + 3 \\ &= 6 \end{aligned}$$

Method 2: Quick application:

$$\lim_{x \rightarrow 3} (x^2 - 2x + 3) = 3^2 - 2 \cdot 3 + 3 = 6$$

Example 2 (page 156): Calculate $\lim_{x \rightarrow 1} \frac{2x}{x^2 + 4}$

$$\begin{aligned} &= \frac{\lim_{x \rightarrow 1} 2x}{\lim_{x \rightarrow 1} x^2 + 4} \\ &= \frac{2}{5} \end{aligned}$$

Method 2 : Nature

$$= \frac{2 \lim_{x \rightarrow 1} x}{\lim_{x \rightarrow 1} x^2 + \lim_{x \rightarrow 1} 4}$$

$$= \frac{2 \cdot 1}{1^2 + 4} = \frac{2}{5}$$

Example 3(page 156): Calculate $\lim_{x \rightarrow 3} \frac{x^2 + 1}{2\sqrt{x}}$

Method 1: Nature

$$\begin{aligned} & \lim_{x \rightarrow 3} \frac{x^2 + 1}{2\sqrt{x}} \\ &= \frac{\lim_{x \rightarrow 3} x^2 + \lim_{x \rightarrow 3} 1}{2 \cdot \lim_{x \rightarrow 3} \sqrt{x}} \end{aligned}$$

$$= \frac{3^2 + 1}{2 \cdot \sqrt{3}} = \frac{5\sqrt{3}}{3}$$

Method 2: Quick application

$$= \frac{3^2 + 1}{2 \cdot \sqrt{3}} = \frac{5}{\sqrt{3}} = \frac{5\sqrt{3}}{3}$$

Example 4(page 156):

a)

$$\begin{aligned} & \lim_{x \rightarrow 2} [5f(x) + (g(x))^2] \\ &= 5 \lim_{x \rightarrow 2} 3 + \lim_{x \rightarrow 2} 4^2 \\ &= 5 \cdot 3 + 4^2 = 31 \end{aligned}$$

b)

$$\begin{aligned} & \lim_{x \rightarrow 2} \frac{f(x) - 4}{g(x)} \\ &= \frac{3 - 4}{4} = -\frac{1}{4} \end{aligned}$$

Method 2: Nature

$$\lim_{x \rightarrow 2} \frac{f(x) - 4}{g(x)} = \frac{\lim_{x \rightarrow 2} f(x) - \lim_{x \rightarrow 2} 4}{\lim_{x \rightarrow 2} g(x)} = \frac{3 - 4}{4} = -\frac{1}{4}$$

Example 5(page 156):

We have a linear equation in two variable, $f(x)$ and $g(x)$:

$$\lim_{x \rightarrow 2} 3f(x) - 2g(x) = 2$$

$$\lim_{x \rightarrow 2} 2f(x) - g(x) = 3$$

$$\begin{aligned} & \iff \begin{cases} \lim_{x \rightarrow 2} 3f(x) - 2 \lim_{x \rightarrow 2} g(x) = 2 \\ \lim_{x \rightarrow 2} 2f(x) - \lim_{x \rightarrow 2} g(x) = 3 \end{cases} \iff \begin{cases} f(x) = 4 \\ g(x) = 5 \end{cases} \\ & \implies \lim_{x \rightarrow 2} \{f(x) + g(x)\} = \lim_{x \rightarrow 2} f(x) + \lim_{x \rightarrow 2} g(x) = 4 + 5 = 9 \end{aligned}$$

Example 1 (Page 158):

$$\lim_{x \rightarrow 2} \frac{x^2 - 4}{x^2 - 3x + 2} \text{ with } x = 2 \implies \text{form } \frac{0}{0}$$

$$\lim_{x \rightarrow 2} \frac{x^2 - 4}{x^2 - 3x + 3} = \frac{(x-2)(x+2)}{(x-2)(x-1)} = \frac{x+2}{x-1} = 4$$

\implies choose B.

Example 2(page 158):

The numerator : $(-1)^2 + (2 \cdot -1) + 1 = 0$

The denominator : $2 \cdot -1 + 2 = 0$

\implies form $\frac{0}{0}$

$$\lim_{x \rightarrow -1} \frac{x^2+2x+1}{2x+2} = \lim_{x \rightarrow -1} \frac{(x+1)^2}{2(x+1)} = \lim_{x \rightarrow -1} \frac{x+1}{2} = \frac{-1+1}{2} = \frac{0}{2} = 0$$

\Rightarrow choose B.

Example 3(page 158):

The numerator: $2 \cdot (\sqrt{3})^2 - 6 = 0$

The denominator: $\sqrt{3} - \sqrt{3} = 0$

\Rightarrow form $\frac{0}{0}$

$$I = \lim_{x \rightarrow \sqrt{3}} \frac{2x^2-6}{x-\sqrt{3}} = \lim_{x \rightarrow \sqrt{3}} \frac{2(x^2-3)}{x-\sqrt{3}} = \lim_{x \rightarrow \sqrt{3}} \frac{2(x-\sqrt{3})(x+\sqrt{3})}{x-\sqrt{3}} = \lim_{x \rightarrow \sqrt{3}} 2 \cdot (x + \sqrt{3}) = 2 \cdot (\sqrt{3} + \sqrt{3}) = 4\sqrt{3}$$

$\Rightarrow a^2 + b^2 = 4^2 + 3^2 = 16 + 9 = 25 \Rightarrow$ choose D.

Example 4(page 158):

The numerator : $1^2 + (3a + 2) \cdot 1 - 3a - 3 = 0$

The denominator: $1 - 1 = 0$

\Rightarrow from $\frac{0}{0}$

We transform the numerator :

$$\begin{aligned} & x^2 + (3a + 2)x - 3a - 3 \\ &= x^2 + 3ax + 2x - 3a - 3 \\ &= (x^2 + 2x - 3) + (3ax - 3a) \\ &= (x - 1)(x + 3) + 3a(x - 1) \\ &= (x - 1)[(x + 3) + 3a] \\ &= (x - 1)(x + 3a + 3) \\ &\Rightarrow \lim_{x \rightarrow 1} \frac{x^2 + (3a+2)x - 3a - 3}{x - 1} = \lim_{x \rightarrow 1} \frac{(x-1)(x+3a+3)}{x-1} = \lim_{x \rightarrow 1} (x + 3a + 3) = 1 + 3a + 3 = 3a + 4 \Rightarrow \text{choose C.} \end{aligned}$$

Example 5(page 158):

\Rightarrow form $\frac{0}{0}$

\Rightarrow form $\sqrt{A} - B \Rightarrow$ using technique "multiplying by the conjugate."

$$\begin{aligned} &\Rightarrow \lim_{x \rightarrow 5} \frac{\sqrt{3x+1}-4}{3-\sqrt{x+4}} = \lim_{x \rightarrow 5} \frac{(\sqrt{3x+1}-4)(\sqrt{3x+1}+4)(3+\sqrt{x+4})}{(\sqrt{3x+1}+4)(3-\sqrt{x+4})(3+\sqrt{x+4})} = \lim_{x \rightarrow 5} \frac{(3x+1-16)(3+\sqrt{x+4})}{(\sqrt{3x+1}+4)[3^2-(x+4)]} = \\ &\lim_{x \rightarrow 5} \frac{(3x-15)(3+\sqrt{x+4})}{(\sqrt{3x+1}+4)(5-x)} = \lim_{x \rightarrow 5} \frac{3(x-5)(3+\sqrt{x+4})}{(\sqrt{3x+1}+4)(5-x)} = \lim_{x \rightarrow 5} \frac{-3(3+\sqrt{x+4})}{\sqrt{3x+1}+4} = \frac{-3(3+\sqrt{5+4})}{\sqrt{3 \cdot 5+1}+4} = -\frac{9}{4} \end{aligned}$$

Example 6(page 158):

\Rightarrow form $\frac{0}{0}$

we know : $\sqrt[3]{1} = 1$

we know : $a^3 + b^3 = (a + b)(a^2 - ab + b^2)$

we know : $a^3 - a^3 = (a - b)(a^2 + ab + b^2)$

$$\begin{aligned} &\Rightarrow \text{we have conjugate expression : } (\sqrt[3]{1+4x})^2 + (\sqrt[3]{1+4x} \cdot 1) + 1^2 \Rightarrow \\ &\lim_{x \rightarrow 0} \frac{\sqrt[3]{1+4x}-1}{x} = \lim_{x \rightarrow 0} \frac{(\sqrt[3]{1+4x}-1) \cdot (\sqrt[3]{1+4x})^2 + (\sqrt[3]{1+4x} \cdot 1) + 1^2}{x \cdot [(\sqrt[3]{1+4x})^2 + (\sqrt[3]{1+4x} \cdot 1) + 1^2]} = \lim_{x \rightarrow 0} \frac{1+4x-1}{x \cdot [(\sqrt[3]{1+4x})^2 + (\sqrt[3]{1+4x} \cdot 1) + 1^2]} = \\ &\lim_{x \rightarrow 0} \frac{4}{(\sqrt[3]{1+4x})^2 + (\sqrt[3]{1+4x} \cdot 1) + 1^2} = \frac{4}{3} \end{aligned}$$

Example 7(page 158):

$$\begin{aligned}
& \frac{1}{2-2} \cdot \left(\frac{1}{2+4} - \frac{1}{2^2+2} \right) \implies \text{form } 0 \cdot \infty \\
& \implies \left(\frac{1}{x+4} - \frac{1}{x^2+x} \right) = \left(\frac{1}{x+4} - \frac{1}{x(x+1)} \right) = \frac{x(x+1)}{(x+4)[x(x+1)]} - \frac{(x+4)}{(x+4)[x(x+1)]} = \\
& \frac{x^2-4}{(x+4)[x(x+1)]} = \frac{(x-2)(x+2)}{(x+4)[x(x+1)]} \\
& \implies \lim_{x \rightarrow 2} \frac{1}{x-2} \cdot \left(\frac{1}{x+4} - \frac{1}{x^2+x} \right) = \lim_{x \rightarrow 2} \frac{1}{x-2} \cdot \left(\frac{(x-2)(x+2)}{(x+4)[x(x+1)]} \right) = \lim_{x \rightarrow 2} \frac{(x-2)(x+2)}{(x-2)(x+4)[x(x+1)]} \\
& = \lim_{x \rightarrow 2} \frac{(x+2)}{(x+4)[x(x+1)]} = \frac{2+2}{(2+4) \cdot [2(2+1)]} = \frac{1}{9}
\end{aligned}$$

Example 8(page 158):

We know : $\lim_{x \rightarrow a} \{f(x) \cdot g(x)\} = \lim_{x \rightarrow a} f(x) \cdot \lim_{x \rightarrow a} g(x) = \alpha \cdot \beta$

$$\implies \lim_{x \rightarrow 2} \frac{(x^2+2x) \cdot f(x)}{x-2} = 9 \iff \lim_{x \rightarrow 2} (x^2+2x) \cdot \lim_{x \rightarrow 2} \frac{f(x)}{x-2} = 9$$

$$\implies \lim_{x \rightarrow 2} \frac{f(x)}{x-2} = \frac{9}{8}$$

$$\implies \lim_{x \rightarrow 2} \frac{(x^3+4x+8) \cdot f(x)}{x-2} = \lim_{x \rightarrow 2} (x^3+4x+8) \cdot \lim_{x \rightarrow 2} \frac{f(x)}{x-2} = 24 \cdot \frac{9}{8} = 27$$

Example 9(page 158):

$$I = \lim_{x \rightarrow 3} \frac{x-3}{\sqrt{x+a+b}} = 6$$

We can see the numerator : $3-3=0 \implies I$ is definitely in the form $\frac{0}{0}$, because the $\frac{0}{0}$ form, after simplification, will result in a finite value.

$$\implies \sqrt{x+a+b} = 0$$

$$\implies \sqrt{3+a+b} = 0$$

$$\implies b = -\sqrt{3+a}$$

$$\begin{aligned}
& \implies \lim_{x \rightarrow 3} \frac{x-3}{\sqrt{x+a+b}} = \lim_{x \rightarrow 3} \frac{x-3}{\sqrt{x+a-\sqrt{3+a}}} = \frac{(x-3) \cdot (\sqrt{x+a} + \sqrt{3+a})}{(\sqrt{x+a}-\sqrt{3+a}) \cdot (\sqrt{x+a} + \sqrt{3+a})} = \lim_{x \rightarrow 3} \frac{(x-3) \cdot (\sqrt{x+a} + \sqrt{3+a})}{(x+a)-(3+a)} = \\
& \lim_{x \rightarrow 3} \frac{(x-3) \cdot (\sqrt{x+a} + \sqrt{3+a})}{(x-3)} = \lim_{x \rightarrow 3} (\sqrt{x+a} + \sqrt{3+a}) = 2\sqrt{3+a} = 6
\end{aligned}$$

$$\implies \sqrt{3+a} = 3$$

$$\implies 3+a=9 \implies a=6 \implies b=-3 \implies a-b=6-(-3)=9$$

Additional practice exercises(page 159):

BON 1:

form $\frac{0}{0}$

$$\implies \lim_{x \rightarrow 1} \frac{x-1}{x^2+2x-3} = \lim_{x \rightarrow 1} \frac{x-1}{(x-1)(x+3)} = \lim_{x \rightarrow 1} \frac{1}{x+3} = \frac{1}{4}$$

BON 2:

form $\frac{0}{0}$

$$\begin{aligned}
& \implies \lim_{x \rightarrow 2} \frac{x^3-8}{x-2} = \lim_{x \rightarrow 2} \frac{x^3-2^3}{x-2} = \lim_{x \rightarrow 2} \frac{(x-2)(x^2+2x+2^2)}{(x-2)} = \lim_{x \rightarrow 2} x^2 + \\
& 2x + 2^2 = 2^2 + 2 \cdot 2 + 4 = 12
\end{aligned}$$

BON 3:

form $\frac{0}{0}$

$$\implies \lim_{x \rightarrow -1} \frac{x^3+2x^2+x}{x^2-1} = \lim_{x \rightarrow -1} \frac{x(x^2+2x+1)}{(x-1)(x+1)} = \lim_{x \rightarrow -1} \frac{x(x+1)^2}{(x-1)(x+1)} = \lim_{x \rightarrow -1} \frac{x(x+1)}{(x-1)} = 0$$

BON 4:

form $\frac{0}{0}$

$$\implies \lim_{x \rightarrow 1} \frac{x-1}{\sqrt{x}-1} = \lim_{x \rightarrow 1} \frac{(x-1)(\sqrt{x}+1)}{(\sqrt{x}-1)(\sqrt{x}+1)} = \lim_{x \rightarrow 1} \frac{(x-1)(\sqrt{x}+1)}{(x-1)} = \lim_{x \rightarrow 1} (\sqrt{x}+1) = 2$$

BON 5:

form $\frac{0}{0}$

$$\implies \lim_{x \rightarrow 1} \frac{\sqrt{x+8}-3}{x^2-1} = \lim_{x \rightarrow 1} \frac{(\sqrt{x+8}-3)(\sqrt{x+8}+3)}{(x-1)(x+1)(\sqrt{x+8}+3)} = \lim_{x \rightarrow 1} \frac{(x-1)}{(x-1)(x+1)(\sqrt{x+8}+3)} =$$

$$\lim_{x \rightarrow 1} \frac{1}{(x+1)(\sqrt{x+8}+3)} = \frac{1}{12}$$

BON 6:

form $\infty \cdot 0 \implies$ convert to form $\frac{0}{0}$

$$\implies \left(\frac{1}{\sqrt{x+1}} - 1 \right) = \frac{1}{\sqrt{x+1}} - \frac{\sqrt{x+1}}{\sqrt{x+1}} = \frac{1-\sqrt{x+1}}{\sqrt{x+1}}$$

$$\implies \lim_{x \rightarrow 0} \frac{1}{x} \left(\frac{1}{\sqrt{x+1}} - 1 \right) = \lim_{x \rightarrow 0} \frac{1}{x} \left(\frac{1-\sqrt{x+1}}{\sqrt{x+1}} \right) = \lim_{x \rightarrow 0} \frac{1-\sqrt{x+1}}{x(\sqrt{x+1})} \implies \text{we have}$$

form $\frac{0}{0}$

$$\implies \lim_{x \rightarrow 0} \frac{1-\sqrt{x+1}}{x(\sqrt{x+1})} = \lim_{x \rightarrow 0} \frac{(1-\sqrt{x+1})(1+\sqrt{x+1})}{x(\sqrt{x+1})(1+\sqrt{x+1})} = \lim_{x \rightarrow 0} \frac{1-(x+1)}{x(\sqrt{x+1})(1+\sqrt{x+1})} = \lim_{x \rightarrow 0} \frac{-x}{x(\sqrt{x+1})(1+\sqrt{x+1})} =$$

$$\lim_{x \rightarrow 0} \frac{-1}{(\sqrt{x+1})(1+\sqrt{x+1})} = -\frac{1}{2}$$

BON 7:

$$I = \lim_{x \rightarrow 2} \frac{f(x)-3x}{x-2} = 3 = c \implies I \text{ have form } \frac{0}{0} \text{ after that, remove the}$$

indeterminate form $\frac{0}{0}$ to get a result of 3, hence, the constant $c = 3$

$$\implies I \text{ Sure have form } \frac{0}{0}$$

$$\implies f(x) - 3x = 0 \implies f(2) = 6$$

$$\implies \lim_{x \rightarrow 2} \frac{[f(x)-3x] \cdot [f(x)+2]}{x^2-4} = \lim_{x \rightarrow 2} \frac{f(x)-3x}{(x-2)} \cdot \lim_{x \rightarrow 2} \frac{f(x)+2}{(x+2)} = 3 \cdot \frac{8}{4} = 6$$

Note:

All the addition, subtraction, multiplication, and division properties of limits as $x \rightarrow a$ are valid only when the two individual limits both exist (and are finite numbers).

BON 8:

$$I = \lim_{x \rightarrow 0} \frac{\sqrt{x^2+ax+b}-a}{\sqrt{x+a}-\sqrt{a-x}} = 1$$

We can see denominator: $\sqrt{0+a}-\sqrt{a-0} = \sqrt{a}-\sqrt{a} = 0 \implies I$ is definitely in the form $\frac{0}{0}$, because the $\frac{0}{0}$ form, after simplification, will result in a finite value.

$$\implies \sqrt{x^2+ax+b}-a = 0$$

$$\iff \sqrt{b}-a = 0$$

$$\implies a = \sqrt{b} \iff b = a^2$$

$$\implies I = \lim_{x \rightarrow 0} \frac{\sqrt{x^2+ax+a^2}-a}{\sqrt{x+a}-\sqrt{a-x}} = \lim_{x \rightarrow 0} \frac{(\sqrt{x^2+ax+a^2}-a)(\sqrt{x^2+ax+a^2}+a)(\sqrt{x+a}+\sqrt{a-x})}{(\sqrt{x+a}-\sqrt{a-x})(\sqrt{x+a}+\sqrt{a-x})(\sqrt{x^2+ax+a^2}+a)} =$$

$$\lim_{x \rightarrow 0} \frac{x(x+a)(\sqrt{x+a}+\sqrt{a-x})}{2x(\sqrt{x^2+ax+a^2}+a)} = \lim_{x \rightarrow 0} \frac{(x+a)(\sqrt{x+a}+\sqrt{a-x})}{2(\sqrt{x^2+ax+a^2}+a)} = \lim_{x \rightarrow 0} \frac{(0+a)(\sqrt{0+a}+\sqrt{a-0})}{2(\sqrt{0^2+a \cdot 0+a^2}+a)} = \frac{2a\sqrt{a}}{4a} =$$

$$\frac{\sqrt{a}}{2} = 1 \implies a = 4 \implies b = 16 \implies a + b = 20$$